rocq/theories/TypeSystem/EnvStructuralRules.v
@@ -627,6 +627,17 @@ Inductive typed_env_structural (env : global_env) (Ω : outlives_ctx) (n : nat)
       contains_lbound_outlives (open_bound_outlives σ bounds) = false ->
       Forall (fun '(a, b) => outlives Ω a b) (open_bound_outlives σ bounds) ->
       typed_env_structural env Ω n Σ (ECallExpr callee args) (open_bound_ty σ ret) Σ'
+  | TES_CallExpr_Forall_Closure :
+      forall Σ Σ1 Σ' callee args u m bounds body env_lt param_tys ret σ,
+      typed_env_structural env Ω n Σ callee (MkTy u (TForall m bounds body)) Σ1 ->
+      ty_core body = TClosure env_lt param_tys ret ->
+      typed_args_env_structural env Ω n Σ1 args
+        (params_of_tys (map (open_bound_ty σ) param_tys)) Σ' ->
+      contains_lbound_lifetime (open_bound_lifetime σ env_lt) = false ->
+      contains_lbound_ty (open_bound_ty σ ret) = false ->
+      contains_lbound_outlives (open_bound_outlives σ bounds) = false ->
+      Forall (fun '(a, b) => outlives Ω a b) (open_bound_outlives σ bounds) ->
+      typed_env_structural env Ω n Σ (ECallExpr callee args) (open_bound_ty σ ret) Σ'
 with typed_args_env_structural (env : global_env) (Ω : outlives_ctx) (n : nat)
     : sctx -> list expr -> list param -> sctx -> Prop :=
   | TESArgs_Nil : forall Σ,
@@ -1660,11 +1671,13 @@ Proof.
         sctx_same_bindings_trans.
     + eauto using typed_args_env_structural_same_bindings,
         sctx_same_bindings_trans.
-    + eauto using typed_args_env_structural_same_bindings,
-        sctx_same_bindings_trans.
-    + eauto using typed_args_env_structural_same_bindings,
-        sctx_same_bindings_trans.
-  - intros env Ω n Σ args ps Σ' Htyped.
+	    + eauto using typed_args_env_structural_same_bindings,
+	        sctx_same_bindings_trans.
+	    + eauto using typed_args_env_structural_same_bindings,
+	        sctx_same_bindings_trans.
+	    + eauto using typed_args_env_structural_same_bindings,
+	        sctx_same_bindings_trans.
+	  - intros env Ω n Σ args ps Σ' Htyped.
     induction Htyped.
     + apply sctx_same_bindings_refl.
     + eapply sctx_same_bindings_trans.
